feat: (wip) impl `Lambda`, pt. 2

Plfl/Lambda.lean
@@ -1,7 +1,12 @@
 -- https://plfa.github.io/Lambda/
 
-def Sym : Type := String deriving Repr
+import Mathlib.Tactic
 
+open String
+
+def Sym : Type := String deriving BEq, DecidableEq, Repr
+
+-- https://plfa.github.io/Lambda/#syntax-of-terms
 inductive Term where
 | var : Sym → Term
 | lam : Sym → Term → Term
@@ -10,32 +15,128 @@ inductive Term where
 | succ : Term → Term
 | case : Term → Term → Sym → Term → Term
 | mu : Sym → Term → Term
-deriving Repr
-
-notation:50 " ƛ " v " ⇒ " d => Term.lam v d
-notation:50 " μ " v " ⇒ " d => Term.mu v d
-notation:max " ? " e " [zero⇒ " o " |succ " n " ⇒ " i " ] " => Term.case e o n i
-infixr:70 " $ " => Term.ap
-notation:max " ο " => Term.zero
-prefix:80 " ι " => Term.succ
-prefix:90 " ` " => Term.var
-
-example : Term := `"foo"
-example : Term := ? `"bar" [zero⇒ ο |succ "n" ⇒ ι ο]
+deriving BEq, DecidableEq, Repr
 
 namespace Term
-  def one : Term := ι ο
-  def two : Term := ι ι ο
+  notation:50 " ƛ " v " : " d => lam v d
+  notation:50 " μ " v " : " d => mu v d
+  notation:max " ? " e " [zero: " o " |succ " n " : " i " ] " => case e o n i
+  -- " · " is `infixl` in the book, but here we choose to use `infixr`.
+  infixr:70 " $ " => ap
+  prefix:80 " ι " => succ
+  prefix:90 " ` " => var
 
-  def add : Term := μ "+" ⇒ ƛ "m" ⇒ ƛ "n" ⇒ ? `"m" [zero⇒ `"n" |succ "m" ⇒ ι (`"+" $ `"m" $ `"n")]
+  def o : Term := zero
+
+  example : Term := `"foo"
+  example : Term := ? `"bar" [zero: o |succ "n" : ι o]
+
+  def one : Term := ι o
+  def two : Term := ι ι o
+
+  def add : Term := μ "+" : ƛ "m" : ƛ "n" : ? `"m" [zero: `"n" |succ "m": ι ((`"+" $ `"m") $ `"n")]
   -- https://plfa.github.io/Lambda/#exercise-mul-recommended
-  def mul : Term := μ "*" ⇒ ƛ "m" ⇒ ƛ "n" ⇒ ? `"m" [zero⇒ ο |succ "m" ⇒ `"+" $ `"n" $ `"*" $ `"m" $ `"n"]
+  def mul : Term := μ "*" : ƛ "m" : ƛ "n" : ? `"m" [zero: o |succ "m": (`"+" $ `"n") $ ((`"*" $ `"m") $ `"n")]
 
   -- Church encoding...
-  def one_c : Term := ƛ "s" ⇒ ƛ "z" ⇒ `"s" $ `"z"
-  def two_c : Term := ƛ "s" ⇒ ƛ "z" ⇒ `"s" $ `"s" $ `"z"
-  def suc_c : Term := ƛ "n" ⇒ ι `"n"
-  def add_c : Term := ƛ "m" ⇒ ƛ "n" ⇒ ƛ "s" ⇒ ƛ "z" ⇒ `"m" $ `"s" $ `"n" $ `"s" $ `"z"
+  def one_c : Term := ƛ "s" : ƛ "z" : `"s" $ `"z"
+  def two_c : Term := ƛ "s" : ƛ "z" : `"s" $ `"s" $ `"z"
+  def succ_c : Term := ƛ "n" : ι `"n"
+  def add_c : Term := ƛ "m" : ƛ "n" : ƛ "s" : ƛ "z" : (`"m" $ `"s") $ ((`"n" $ `"s") $ `"z")
   -- https://plfa.github.io/Lambda/#exercise-mul%E1%B6%9C-practice
-  def mul_c : Term := ƛ "m" ⇒ ƛ "n" ⇒ ƛ "s" ⇒ ƛ "z" ⇒ `"m" $ (`"n" $ `"s") $ `"z"
+  def mul_c : Term := ƛ "m" : ƛ "n" : ƛ "s" : ƛ "z" : `"m" $ (`"n" $ `"s") $ `"z"
 end Term
+
+-- https://plfa.github.io/Lambda/#values
+inductive Value : Term → Prop where
+| lam : Value (ƛ v : d)
+| zero: Value o
+| succ: Value n → Value (ι n)
+
+-- https://plfa.github.io/Lambda/#substitution
+namespace Term
+  /--
+  `x.subst y v` substitutes term `v` for all free occurrences of variable `y` in term `x`.
+  -/
+  def subst : Term → Sym → Term → Term
+  | ` x, y, v => if x = y then v else ` x
+  | ƛ x : n, y, v => if x = y then ƛ x : n else ƛ x : n.subst y v
+  | ap l m, y, v => l.subst y v $ m.subst y v
+  -- `.o` means that `o` is not a new binding, but a constant.
+  -- See: https://leanprover.github.io/theorem_proving_in_lean4/induction_and_recursion.html?highlight=inac#inaccessible-patterns
+  | .o, _, _ => o 
+  | ι n, y, v => ι (n.subst y v)
+  | ? l [zero: m |succ x: n], y, v => if x = y
+      then ? l.subst y v [zero: m.subst y v |succ x: n]
+      else ? l.subst y v [zero: m.subst y v |succ x: n.subst y v]
+  | μ x : n, y, v => if x = y then μ x : n else μ x : n.subst y v
+
+  notation:90 x " [ " y " := " v " ] " => subst x y v
+
+  -- https://plfa.github.io/Lambda/#examples
+  example
+  : (ƛ "z" : (`"s" $ `"s") $ `"z")["s" := succ_c]
+  = (ƛ "z" : (succ_c $ succ_c) $ `"z") := rfl
+
+  example : ((succ_c $ succ_c) $ `"z")["z" := o] = (succ_c $ succ_c) $ o := rfl
+  example : (ƛ "x" : `"y")["y" := o] = (ƛ "x" : o) := rfl
+  example : (ƛ "x" : `"x")["x" := o] = (ƛ "x" : `"x") := rfl
+  example : (ƛ "y" : `"y")["x" := o] = (ƛ "y" : `"y") := rfl
+
+  -- https://plfa.github.io/Lambda/#quiz
+  example
+  : (ƛ "y" : `"x" $ (ƛ "x" : `"x"))["x" := o]
+  = (ƛ "y" : o $ (ƛ "x" : `"x"))
+  := rfl
+
+  -- https://plfa.github.io/Lambda/#reduction
+  /--
+  `Reduce t t'` says that `t` reduces to `t'`.
+  -/
+  inductive Reduce : Term → Term → Prop where
+  | ξ_ap₁ : Reduce l l' → Reduce (l $ m) (l' $ m)
+  | ξ_ap₂ : Value v → Reduce m m' → Reduce (v $ m) (v $ m')
+  | β_lam : Value v → Reduce ((ƛ x : n) $ v) (n[x := v])
+  | ξ_succ : Reduce m m' → Reduce (ι m) (ι m')
+  | ξ_case : Reduce l l' → Reduce (? l [zero: m |succ x : n]) (? l' [zero: m |succ x : n])
+  | β_zero : Reduce (? o [zero: m |succ x : n]) m
+  | β_succ : Value v → Reduce (? ι v [zero: m |succ x : n]) (n[x := v])
+  | β_mu : Reduce (μ x : m) (m[x := μ x : m])
+
+  infix:40 " —→ " => Reduce
+end Term
+
+namespace Term.Reduce
+  -- https://plfa.github.io/Lambda/#quiz-1
+  example : ((ƛ "x" : `"x") $ (ƛ "x" : `"x")) —→ (ƛ "x" : `"x") := by
+    apply β_lam; exact Value.lam
+
+  example
+  : (((ƛ "x" : `"x") $ (ƛ "x" : `"x")) $ (ƛ "x" : `"x"))
+  —→ ((ƛ "x" : `"x") $ (ƛ "x" : `"x"))
+  := by
+    apply ξ_ap₁; apply β_lam; exact Value.lam
+
+  example
+  : ((two_c $ succ_c) $ o)
+  —→ ((ƛ "z" : succ_c $ succ_c $ `"z") $ o)
+  := by
+    unfold two_c; apply ξ_ap₁; apply β_lam; exact Value.lam
+
+  -- https://plfa.github.io/Lambda/#reflexive-and-transitive-closure
+  /--
+  A reflexive and transitive closure,
+  defined as a sequence of zero or more steps of the underlying relation `—→`.
+  -/
+  inductive Clos : Term → Term → Prop where
+  | step : (m —→ n) → Clos m n
+  | refl : Clos m m
+  | trans : Clos l m → Clos m n → Clos l n
+
+  infix:20 " —↠ " => Clos
+
+  instance preorder : Preorder Term where
+    le := Clos
+    le_refl := by simp [Clos.refl]
+    le_trans := by intros; apply Clos.trans <;> trivial
+end Reduce
